LTL/LTL.v
@@ -1,3 +1,0 @@
-(* LTL/LTL.v *)
-From LTL Require Export Syntax Semantics.
-Local Open Scope LTL_scope.
